\documentclass{ximera}

\input{../../preamble.tex}


\author{Jim Talamo}

\outcome{Find a tangent plane to the graph of a function.}

\begin{document}

\begin{exercise}
 
Which of the following is the equation of the tangent plane at the point on the surface $z=(2x-1)^2(y+4)$ where $x=1$ and $y=-2$?

\begin{multipleChoice}
\choice{$8x+y-z = -4$}
\choice[correct]{$8x+y-z = 4$}
\choice{$8x+y+z = -8$}
\choice{$4x+y-z = 0 $}
\choice{$2x+y-z = 2$}
\choice{none of these}
\end{multipleChoice}

\begin{exercise}
Does the point $(1,-2)$ lies on the curve $2x+y^2=6$?  \wordChoice{\choice[correct]{Yes}\choice{No}}

Now, let's find the curve on the surface associated to this curve in the domain. Set $y(t)=2t$.  A parameterization of the curve $2x+y^2=6$ in the $xy$- plane is

\[
\vec{r}(t) = \vector{\answer{3-2t^2},2t},
\]

and a parameterization of the associated curve on the surface is 

\[
\vec{R}(t) = \vector{\answer{3-2t^2},2t, \answer{(-4t^2+5)^2\cdot(2t+4) } }.
\]

\begin{exercise}
Find a parametric description of the tangent line to the curve in the previous part at the point $(1,-2,2)$.

\[
\vec{l}(t) = \vector{\answer{4t+1 } , \answer{2t-2} , \answer{34t+2} }
\]

\begin{hint}
What must $t$ be so $(x(t),y(t),z(t)) = (1,-2,2)$?  You can use any of the components of $\vec{R}(t)$ (although one allows for an efficient computation) to find that $t=\answer{-1}$.

\begin{hint}
A vector parallel to the tangent line is $\vec{R}'(-1)$.  

\begin{align*}
\vec{R}'(t) &= \vector{\answer{-4t},\answer{2},\answer{-16(-4t^2+5)(2t^2+4t) +2(-4t^2+5)^2 }} \\
\vec{R}'(-1) &= \vector{\answer{4},\answer{2},\answer{34}} \\
\end{align*}

Use $\vec{l}(t) =\vec{v}t+\vec{P}_0$ where $P_0 = (1,-2,2)$.
\end{hint}
\end{hint}

To determine whether the tangent line $\vec{l}(t)$ lies on the tangent plane, we must check whether

\[
8\big[x(t)\big]+\big[y(t)\big]-\big[z(t)\big] = 4
\]

for all $t$.  

Does the tangent line lie on the tangent plane?  \wordChoice{\choice[correct]{Yes}\choice{No}}

\begin{feedback}[correct]
Note that 

\begin{align*}
8\big[x(t)\big]+\big[y(t)\big]-\big[z(t)\big] & = 8\big[4t+1\big]+\big[2t-2\big]-\big[34t+2\big]\\
&= 32t+8+2t-2-34t-2 \\
&=4
\end{align*}
\end{feedback}


\end{exercise}
\end{exercise}
\end{exercise}
\end{document}
