\documentclass{ximera}
\input{../../preamble.tex}
\author{Jim Talamo}
\license{Creative Commons 3.0 By-NC}
\outcome{Verify solutions to differential equations}
\begin{document}


\begin{exercise}
Consider the initial value problem: $y' +x^3y^2 = 0, \quad y(2)=1$.

Let $f(x)$ be a solution to this initial value problem.

Then, the equation of the tangent line at $x=2$ to $y=f(x)$ is:

\[
y = \answer{-8x+17}
\]

\begin{hint}
We need a point and a slope, but we do not have to solve the differential equation to find these.

Substituting $x=\answer{2}$ and $y=\answer{1}$ into the equation gives $y' = \answer{-8}$.  

Using the point-slope form of a tangent line, we find:

\begin{align*}
y-y_0 &= m_{tan} \left(x-x_0\right) \\
y-\answer{1} &= \answer{-8} \left(x-\answer{2}\right)
\end{align*}
\end{hint}

\begin{exercise}

Find $f''(2)$.

\[
f''(2) = \answer{116 }
\]
\begin{hint}
Without the initial value problem, how could we find $f''(2)$?

\begin{multipleChoice}
\choice[correct]{Use the differential equation to find $f''(2)$.  Then, differentiate both sides of the differential equation and substitute known values.}
\choice{It is impossible to determine $f''(2)$ without solving the differential equation.}
\end{multipleChoice}

From the differential equation, we find $f'(1) = \answer{-8}$.  We can now differentiate both sides with respect to $x$ to obtain an expression for $y''$.  Note that when we differentiate the $x^3y^2$ term, we will need:

\begin{selectAll}
\choice[correct]{product rule}
\choice{quotient rule}
\choice[correct]{chain rule}
\end{selectAll}

Performing the differentiation, we find $\dd[y]{x} (x^3y^2) = \answer{3x^2} \cdot y^2 + 2x^3yy'$, so after differentiating both sides:

\begin{align*}
\dd{x}(y' +x^3y^2) &= \dd{x}(0) \\
y''+3x^2y^2+2x^3yy' &= 0\\
\end{align*}

(make sure you understand how to perform the implicit differentiation!)

To find $y''(2)$, substitute $x=\answer{2}$, $y=\answer{1}$, and $y'(2) = \answer{-8}$ into the equation.
\end{hint}

\end{exercise}
\end{exercise}

\end{document}