\documentclass{ximera}

\input{../../preamble.tex}

\author{Jim Talamo}
\license{Creative Commons 3.0 By-bC}


\outcome{}


\begin{document}

\begin{exercise}
Suppose that we want to find:

\[
\lim_{x \to 0} \frac{e^{x^3}-1}{2x \sin(x^2)}
\]

%Add trying to use L'H

We could attempt to apply L'Hopital's rule here since substitution gives the indeterminate form $\frac{0}{0}$, but this would not be a particularly efficient way to solve the problem!  A better strategy will be to use Taylor series:


\paragraph{Step 1:} Let's start by writing out the sum of the first several terms in the series centered at $x=0$ (where the limit is to be evaluated) for the numerator and the denominator:

\begin{exercise}
For the numerator, the sum of the first three nonzero terms in the Taylor series centered at $x=0$ is:

\[
e^{x^3}-1 = \answer{x^3+\frac{1}{2}x^6+\frac{1}{6}x^9} +\cdots
\]

\begin{hint}
Use the usual composition rule to find the first several terms in the series for $e^{x^3}$:

\begin{align*}
e^x &= 1+x+\frac{1}{2!}x^2+\frac{1}{3!}x^3+\cdots \\
e^{x^3} &= 1+(x^3)+\frac{1}{2!}(x^3)^2+\frac{1}{3!}(x^3)^3+\cdots \\
&= \answer{1+x^3+\frac{1}{2}x^6+\frac{1}{6}x^9}+\cdots \\
\end{align*}
Now, subtract $1$ from both sides.
\end{hint}
\end{exercise}


\begin{exercise}
For the denominator, the sum of the first three nonzero terms in the Taylor series centered at $x=0$ is:

\[
2x \sin(x^2) = \answer{2x^3-\frac{1}{3}x^7+\frac{1}{60}x^{11}} +\cdots
\]

\begin{hint}
Use the usual composition rule to find the first several terms in the series for $\sin(x^2)$:

\begin{align*}
\sin(x) &= x-\frac{1}{3!}x^3+\frac{1}{5!}x^5+\cdots \\
\sin(x^2) &= (x^2)-\frac{1}{3!}(x^2)^3+\frac{1}{5!}(x^2)^5+\cdots \\
&= \answer{x^2-\frac{1}{6}x^6+\frac{1}{120}x^{10}}+\cdots \\
\end{align*}
Now, multiply by $2x$.
\end{hint}
\end{exercise}


\begin{exercise}
Note that we may need more terms, but we can always exhibit more if necessary.  

\paragraph{Step 2:} Now that we have the series, let's substitute them into the limit:

\[
\lim_{x \to 0} \frac{e^{x^3}-1}{x \sin(x^2)} = \lim_{x \to 0} \frac{  \answer{x^3+\frac{1}{2}x^6+\frac{1}{6}x^9} +\cdots}{\answer{2x^3-\frac{1}{3}x^7+\frac{1}{60}x^{11}} +\cdots}
\]

\paragraph{Step 3:} We can proceed by factoring out the dominant terms from the numerator and denominator:

As $x \to 0$, the dominant power of $x$ in the numerator is $x^{\answer{3}}$.

As $x \to 0$, the dominant power of $x$ in the denominator is $x^{\answer{3}}$.

\begin{exercise}
We can thus write:
\[
L = \lim_{x \to 0} \frac{ x^3+\frac{1}{2}x^6+\frac{1}{6}x^9 +\cdots}{x^3-\frac{1}{6}x^7+\frac{1}{120}x^{11} +\cdots}  = \lim_{x \to 0} \frac{ x^3 \cdot \left[\answer{1+\frac{1}{2}x^3+\frac{1}{6}x^6} +\cdots\right]}{x^3 \cdot \left[\answer{1-\frac{1}{6}x^4+\frac{1}{120}x^{8}} +\cdots\right]}.
\]

\begin{exercise}
 Now, since we took out the dominant power of $x$ in both the numerator and denominator separately, the limits of the functions inside of the square brackets will be constant.  Indeed, we can write the limit as:

\[
L = \lim_{x \to 0} \frac{x^3}{x^3} \cdot \frac{\left[1+\frac{1}{2}x^3+\frac{1}{6}x^6+\cdots \right]}{\left[2-\frac{1}{3}x^4+\frac{1}{60}x^8 +\cdots \right]}
\]

\paragraph{Step 4:} Simplify the expression above, then substitute in $x=0$ to find that the limit is $\answer{\frac{1}{2}}$.


\end{exercise}
\end{exercise}
\end{exercise}
\end{exercise}
\end{document}
