\documentclass{ximera}
\input{../../preamble.tex}
\author{Bart Snapp\and Nela Lakos}
\license{Creative Commons 3.0 By-NC}
\outcome{Use the quotient rule to calculate derivatives.}
\begin{document}
\begin{exercise}
Let $f(x) = \frac{ 2x+1}{5x-3}$. Compute:
\[
f'(x)
\begin{prompt}= \frac{ 2(\answer{5x-3})-(2x+1)(\answer{5})}{(5x-3)^2}= {\frac{ \answer{-11}}{(5x-3)^2}}\end{prompt}
\]
\end{exercise}
\begin{exercise}
Let $f(x) = \frac{ 2x^3+1}{\sin{x}-3}$. Compute:
\[
f'(x)
\begin{prompt}= \frac{ 6x^2(\answer{\sin{x}-3})-(2x^3+1)\answer{\cos{x}}}{(\sin{x}-3)^2}\end{prompt}
\]
\end{exercise}
\begin{exercise}
Let $f(x) = \frac{ 4xe^x-2}{5x-1}$. Compute:
\[
f'(x)
\begin{prompt}= \frac{ (\answer{4e^x+4xe^x})(5x-1)-(\answer{4xe^x-2})5}{(5x-1)^2}\end{prompt}
\]
\end{exercise}
\begin{exercise}
Let $f(x) = \frac{ x^2\sin{x}-x}{4x+3}$. Compute:
\[
f'(x)
\begin{prompt}= \frac{ (\answer{2x\sin{x}+x^2\cos{x}-1})(4x+3)-(\answer{x^2\sin{x}-x})4}{(4x+3)^2}\end{prompt}
\]
\end{exercise}
\end{document}