\documentclass{ximera}

\input{../../preamble.tex}

\author{Jim Talamo}
\license{Creative Commons 3.0 By-bC}


\outcome{}


\begin{document}

\begin{exercise}
Given that $\arctan(x) = \sum_{k=0}^{\infty} \frac{(-1)^k}{2k+1}x^{2k+1}$, find $ \lim_{x \to 0} \frac{\arctan(3x^2)}{\cos(x)-1}
$

The limit is $\answer{-6}$.

(Use $\infty$ or $-\infty$ where appropriate or ``DNE'' if the limit otherwise does not exist)

\begin{hint}
We can use a similar procedure as before:

\paragraph{Step 1:} Let's start by writing out the sum of the first several terms in the series centered at $x=0$ (where the limit is to be evaluated) for the numerator and the denominator:

\begin{question}
For the numerator, we use the usual composition rule to find sum of the first three nonzero terms in the series for $\arctan(3x^2)$:

\begin{align*}
\arctan(x) &= \answer{x-\frac{1}{3}x^3+\frac{1}{5}x^5}+\ldots \\
\arctan(3x^2) &= \answer{(3x^2)-\frac{1}{3}(3x^2)^3+\frac{1}{5}(3x^2)^5}+\ldots \\
&= \answer{3x^2-9x^6+\frac{243}{5}x^{10}}+\ldots \\
\end{align*}
\end{question}


\begin{question}
For the denominator, the sum of the first three nonzero terms in the Taylor series centered at $x=0$ is:

\[
\cos(x)-1 = \answer{-\frac{1}{2!}x^2+\frac{1}{4!}x^4-\frac{1}{6!}x^6} +\ldots
\]

\end{question}


\begin{question}
Note that we may need more terms, but we can always exhibit more if necessary.  

\paragraph{Step 2:} Now that we have the series, let's substitute them into the limit:

\[
\lim_{x \to 0} \frac{\arctan(3x^2)}{\cos(x)-1} = \lim_{x \to 0} \frac{\answer{3x^2-9x^6+\frac{243}{5}x^{10}}+\ldots}{ \answer{-\frac{1}{2!}x^2+\frac{1}{4!}x^4-\frac{1}{6!}x^6} +\ldots}
\]

\paragraph{Step 3:} We can proceed by factoring out the dominant terms from the numerator and denominator:

As $x \to 0$, the dominant power of $x$ in the numerator is $x^{\answer{2}}$.

As $x \to 0$, the dominant power of $x$ in the denominator is $x^{\answer{2}}$.

\begin{question}
We can thus write:
\[
L = \lim_{x \to 0} \frac{3x^2-9x^6+\frac{243}{5}x^{10}+\ldots}{-\frac{1}{2!}x^2+\frac{1}{4!}x^4-\frac{1}{6!}x^6 +\ldots}  = \lim_{x \to 0} \frac{ x^2 \cdot \left[\answer{3-9x^4+\frac{243}{5}x^8+\ldots} \right]}{x^2 \cdot \left[\answer{-\frac{1}{2!}+\frac{1}{4!}x^2-\frac{1}{6!}x^4} +\ldots\right]}
\]

\begin{question}
 Now, since we took out the dominant power of $x$ in both the numerator and denominator separately, the limits of the functions inside of the square brackets will be constant.  Indeed, we can write the limit as:

\[
L = \lim_{x \to 0} \frac{x^2}{x^2} \cdot \frac{\left[3-9x^4+\frac{243}{5}x^8+\ldots\right]}{\left[-\frac{1}{2!}+\frac{1}{4!}x^2-\frac{1}{6!}x^4 +\ldots \right]}
\]

\paragraph{Step 4:} Simplify the expression above, then substitute in $x=0$ to find that the limit is $\answer{-6}$.


\end{question}
\end{question}
\end{question}
\end{hint}
\end{exercise}
\end{document}
