\documentclass{ximera}

\input{../preamble.tex}
\title{Precalculus Review - Section 1 Exercises}

\begin{document}
\begin{abstract}
%
\end{abstract}
\maketitle

\begin{exercise}
Describe the following sets of real numbers in interval notation:
\begin{enumerate}
	\item $\{ x \in \RR \, | \, 4 \leq x \leq 7 \} = \answer[format=string]{[} \answer{4},\answer{7} \answer[format=string]{ ] }$
	\item All real numbers smaller than 3 $= \answer[format=string]{(} \answer{-\infty},\answer{3} \answer[format=string]{ ) }$
	\item $\displaystyle \{ x \in \RR \, | \,  x \leq -31 \} = \answer[format=string]{(} \answer{-\infty},\answer{-31} \answer[format=string]{ ] }$
	\item All real numbers $= \answer[format=string]{(} \answer{-\infty},\answer{\infty} \answer[format=string]{ ) }$
\end{enumerate}
\end{exercise}

\begin{exercise}
\begin{enumerate}
	\item $|\pi|=\answer{\pi}$
	\item $-\left\lvert -\frac{1}{2} \right\rvert=\answer{-\frac{1}{2}}$
	\item $|-0.33|=\answer{0.33}$.
	\item The distance between $-3$ and $-4$ on the number line is: $\answer{1}$
\end{enumerate}
\end{exercise}

\begin{exercise} Compute the following:
\begin{enumerate}
	\item $\left(-3\right)^4 = \answer{81}$.
	\item $4^{-3} = \answer{\frac{1}{64}}$.
	\item $0^{-3} = \answer{\textrm{Does not exist}}$.
	\item $\left( \frac{1}{2} \right)^{-3} = \answer{8}$.
\end{enumerate}
\end{exercise}

\begin{exercise} Expand the following:
\begin{enumerate}
	\item $(x-4)(2x^3+x)=\answer{2x^4-8x^3+x^2-4x}$
	\item $(y-4)^2=\answer{y^2-8y+16}$
	\item $\left(x^3+y^2\right)^2=\answer{x^6+2x^3y^2+y^4}$
	\item $(x^2-12)(x^2+12)=\answer{x^4-144}$
	\item $\left(x^2-x+1\right)(3x-4) = \answer{3x^3-7x^2+7x+4}$.
	\item $\left(2xy-y^2\right)^2 = \answer{4x^2 y^2 - 4 xy^3 + y^4}$.
	\item $\left(x^2-0.2\right)^2 = \answer{x^4 - 0.4 x^2 + 0.04}$.
	\item $x\left(x^3-1\right)\left(x^3+1\right) = \answer{x^7 - x}$.
\end{enumerate}
\end{exercise}

\begin{exercise} Factor the following expressions:
\begin{enumerate}
	\item $x^2 + 3x - 10 = \answer{(x+5)(x-2)}$
	\item $2x^2+7x-4 = \answer{(2x-1)(x+4)}$
	\item $2x^2+2x-24 = \answer{2(x-3)(x+4)}$
	\item $x^4-1 = \answer{(x^2+1)(x-1)(x+1)}$
	\item $x^4-x^2 = \answer{x^2(x+1)(x-1)}$
	\item $x^5-x = \answer{x(x^2+1)(x+1)(x-1)}$
\end{enumerate}
\end{exercise}

\begin{exercise} Evaluate, if possible, the following expressions. If the expression is undefined, write DNE.
	\begin{enumerate}
		\item $\sqrt[3]{-125}=\answer{-5}$
		\item $\sqrt[5]{0}=\answer{0}$
		\item $-\sqrt[3]{64}=\answer{-4}$
		\item $\sqrt{-32}=\answer[format=string]{DNE}$
		\item $\sqrt{\frac{9}{4}}=\answer{\frac{3}{2}}$
	\end{enumerate}
\end{exercise}

\begin{exercise}Simplify or evaluate each of the following:
\begin{enumerate}
	\item $\sqrt[3]{\frac{-125}{64}} = \answer{-\frac{5}{4}}$.
	\item $\frac{\sqrt{100}}{\sqrt{200}} = \answer{\frac{1}{\sqrt{2}}}$.
	\item $\left(\sqrt{2} + \sqrt{3}\right)^2 = \answer{5+2\sqrt{6}}$.
	\item $\left(\sqrt{2}+\sqrt{3}\right)\left(\sqrt{2}-\sqrt{3}\right) = \answer{-1}$.
	\item $\left( \frac{4}{9} \right)^{-3/2} = \answer{\frac{27}{8}}$.
\end{enumerate}
\end{exercise}

\begin{exercise}Simplify
\begin{enumerate}
	\item $\frac{x^3-27}{x^2-9} = \frac{\answer{x^2+3x+9}}{\answer{x+3}}$
	\item $\frac{x^4-x^2}{2x^2+3x+1} = \frac{\answer{x^2(x-1)}}{\answer{(2x+1)}}$
	\item $\frac{1-\frac{3}{x}}{1-\frac{6}{x}+\frac{9}{x^2}} = \frac{\answer{x}}{\answer{x-3}}$
	\item{ Simplify $\frac{1+\frac{1}{x-1}}{1-\frac{1}{x-1}} = \frac{\answer{x}}{\answer{x-2}}$}
	\item{ Simplify (find the common denominator) $\displaystyle \frac{3}{x} + \frac{4}{x-1} + \frac{5}{x+1} = \frac{\answer{12x^2-x-3}}{\answer{x^3-x}}$}
\end{enumerate}
\end{exercise}

\end{document}
