\documentclass{ximera}
\input{../../preamble.tex}
\author{Jim Talamo}
\license{Creative Commons 3.0 By-NC}
\outcome{Verify solutions to differential equations}
\begin{document}


\begin{exercise}
Consider the initial value problem: $y' +2xy = 0, \quad y(1)=2$.

Without the initial value problem, how could we find $y''(1)$?

\begin{multipleChoice}
\choice[correct]{Use the differential equation to find $y'(1)$.  Then, differentiate both sides of the differential equation and substitute known values.}
\choice{It is impossible to determine $y''(1)$ without solving the differential equation.}
\end{multipleChoice}

We find $y''(1) = \answer{4} $

\begin{hint}
From the differential equation, we find $y'(1) = \answer{-4}$.  We can now differentiate both sides with respect to $x$ to obtain an expression for $y''$.  Note that when we differentiate the $2xy$ term, we will need:

\begin{selectAll}
\choice[correct]{product rule}
\choice{quotient rule}
\choice[correct]{chain rule}
\end{selectAll}

Performing the differentiation, we find $\dd[y]{x} (2xy) = \answer{2}y + 2x \answer{y'}$, so after differentiating both sides:

\begin{align*}
\dd{x}(y' +2xy) &= \dd{x}(0) \\
\answer{y''+2y+2xy'} &= 0\\
\end{align*}

To find $y''(1)$, substitute $x=\answer{1}$, $y=\answer{2}$, and $y'(1) = \answer{-4}$ into the equation.
\end{hint}

\begin{exercise}
We can also solve the initial value problem first.  Doing so, we find that the solution is:

\[
y = 2 e^{1-x^2}
\]

Differentiating, we find:

\begin{align*}
y' &= \answer{-4xe^{1-x^2}} \\
y'' &= \answer{-4e^{1-x^2}+8x^2e^{1-x^2}}
\end{align*}

Hence, $y''(1) = \answer{4}$.
\end{exercise}

\end{exercise}

\end{document}